# å®šç§¯åˆ†çš„è®¡ç®—

## å¯¹ç§°æ€§çš„åº”ç”¨

### å¯¹ä¸€èˆ¬å‡½æ•°
$$
\begin{align}
\int_a^b f(x)\text{d}x&=\int_a^b f(a+b-x)\text{d}x \\
\int_0^a f(x)\text{d}x&=\int_0^a f(a-x)\text{d}x \\ 
\int_a^b f(x)\text{d}x&=\int_a^{\frac{(a+b)}2} [f(x)+f(a+b-x)]\text{d}x \\
\int_0^a f(x)\text{d}x&=\int_0^{\frac a2} [f(x)+f(a-x)]\text{d}x \\
\end{align}
$$
è¿™å…¶å®ç›¸å½“äºæŠŠå³åŠè¾¹åŒºé—´åŠ åˆ°å·¦åŠè¾¹æ¥äº†ã€‚ä¸‹é¢ç»™å‡ºå…¶ä¸€äº›ç‰¹ä¾‹

### å¯¹æœ‰å¥‡å¶æ€§çš„å‡½æ•°

è‹¥ $f(x)=f(a+b-x)$ï¼Œå¯¹åº”äºå¶å‡½æ•°ï¼Œæœ‰ï¼š
$$
\int_a^b f(x)\text{d}x=2\int_a^{\frac{(a+b)}2} f(x)\text{d}x
$$
è‹¥ $f(x)=-f(a+b-x)$ï¼Œå¯¹åº”äºå¥‡å‡½æ•°ï¼Œæœ‰ï¼š
$$
\int_a^b f(x)\text{d}x=\int_a^{\frac{(a+b)}2} [f(x)+f(a+b-x)]\text{d}x=0
$$
ç”»ä¸€ä¸‹å›¾ä¼šå¥½ç†è§£å¾ˆå¤š

### æ¢å…ƒæ³•æ±‚è§£å®šç§¯åˆ†

- [ ] æ¢å…ƒæ³•æ±‚è§£å®šç§¯åˆ† ğŸ“… 2026-01-07